Generalize refinement proofs to allow more flexible forms of translation.
This commit generalizes the generic adequacy theorems so that the notion of
compilation/translation between layers doesn't have to be given by a
deterministic function from procs at one layer to procs at the lower layer.

The Goose-specific version is updated to exploit this to handle translations
where we map a sequence of operations to another sequence, specified by giving
a compilation relation between procs.

It was convenient to also generalize certain intermediary proofs to not
necessarily require that refinement imply *exact* equality of return values, or
even that return values be of the same type. The final derived theorems for
Goose and ExMach do use a notion of refinement that implies exact equality of
return values, but going forward we will need this more flexible form of
refinement to reason about data abstraction/private data types.

src/CSL/RefinementAdequacy.v
@@ -13,9 +13,9 @@ Unset Implicit Arguments.
 Import RelationNotations.
 Require Import Helpers.RelationAlgebra.
 
-Definition wp_recovery_refinement {T R OpTa OpTc} Σ (Λa: Layer OpTa) (Λc: Layer OpTc)
+Definition wp_recovery_refinement {Ta Tc R OpTa OpTc} Σ (Λa: Layer OpTa) (Λc: Layer OpTc)
         `{invPreG Σ} `{cfgPreG OpTa Λa Σ}
-        (ea: proc OpTa T) (ec: proc OpTc T) (rec: proc OpTc R) (σ1a: State Λa) σ1c φ φrec E k :=
+        (ea: proc OpTa Ta) (ec: proc OpTc Tc) (rec: proc OpTc R) (σ1a: State Λa) σ1c φ φrec E k :=
   Nat.iter k (λ P, |==> ▷ P)%I
     ((⌜ nclose sourceN ⊆ E ⌝ ∧
              ∃ (φinv : forall {_ : @cfgG OpTa Λa Σ}, State Λc → iProp Σ),
@@ -25,8 +25,8 @@ Definition wp_recovery_refinement {T R OpTa OpTc} Σ (Λa: Layer OpTa) (Λc: Lay
              (source_ctx' ([existT _ ea], (snd σ1a)) ∗ O ⤇ ea ∗ source_state (snd σ1a))
                ={⊤}=∗
                stateI σ1c
-               ∗ WP ec @ NotStuck; ⊤ {{ v, O ⤇ of_val v
-                    ∗ (∀ σ2c, stateI σ2c ={⊤,E}=∗ ∃ σ2a, source_state σ2a ∗ φ v σ2a (snd σ2c))}}
+               ∗ WP ec @ NotStuck; ⊤ {{ vc, ∃ (va: Ta), O ⤇ of_val va
+                    ∗ (∀ σ2c, stateI σ2c ={⊤,E}=∗ ∃ σ2a, source_state σ2a ∗ φ va vc σ2a (snd σ2c))}}
                     ∗ (∀ σ2c, stateI σ2c ={⊤,E}=∗ φinv σ2c)
         ∗
         □ (∀ `{Hinv : invG Σ} `{Hcfg: cfgG OpTa Λa Σ} σ1c σ1c'
@@ -40,20 +40,24 @@ Definition wp_recovery_refinement {T R OpTa OpTc} Σ (Λa: Layer OpTa) (Λc: Lay
                ∗ (∀ σ2c, stateI σ2c ={⊤,E}=∗ φinv σ2c))))))%I.
 
 
-Fixpoint wp_proc_seq_refinement {T R OpTa OpTc} {Σ} (Λa: Layer OpTa) (Λc: Layer OpTc)
+Fixpoint wp_proc_seq_refinement {Ta Tc R OpTa OpTc} {Σ} (Λa: Layer OpTa) (Λc: Layer OpTc)
         `{invPreG Σ} `{cfgPreG OpTa Λa Σ}
-        (es: proc_seq OpTa T) (rec: proc OpTc R) (f: ∀ T, proc OpTa T → proc OpTc T)
-        (σ1a: State Λa) σ1c φ E {struct es} : iProp Σ :=
-  match es with
-  | Proc_Seq_Nil v => (φ v σ1a σ1c)%I
-  | @Proc_Seq_Bind _ _ T0 e es' =>
-    wp_recovery_refinement Σ Λa Λc e (f _ e) rec σ1a σ1c
-      (λ v σ2a σ2c, ∀ σ2c' (Hfinish: Λc.(finish_step) σ2c (Val σ2c' tt)),
+        (esa: proc_seq OpTa Ta) (esc: proc_seq OpTc Tc) (rec: proc OpTc R)
+        (σ1a: State Λa) σ1c φ E {struct esa} : iProp Σ :=
+  match esa, esc with
+  | Proc_Seq_Nil va, Proc_Seq_Nil vc => (φ va vc σ1a σ1c)%I
+  | @Proc_Seq_Bind _ _ T0a ea esa,
+    @Proc_Seq_Bind _ _ T0c ec esc =>
+    wp_recovery_refinement Σ Λa Λc ea ec rec σ1a σ1c
+      (λ (va: T0a) (vc: T0c)  σ2a σ2c, ∀ σ2c' (Hfinish: Λc.(finish_step) σ2c (Val σ2c' tt)),
           ∃ σ2a' (Hfinisha: Λa.(finish_step) σ2a (Val σ2a' tt)),
-          wp_proc_seq_refinement Λa Λc (es' (Normal (existT T0 v)))
-                                         rec f (1, σ2a') (1, σ2c') φ E)%I
-      (λ σ2a σ2c, wp_proc_seq_refinement Λa Λc (es' (Recovered (existT _ tt)))
-                                         rec f (1, σ2a) (1, σ2c) φ E) E O
+          wp_proc_seq_refinement Λa Λc (esa (Normal (existT T0a va)))
+                                       (esc (Normal (existT T0c vc)))
+                                         rec (1, σ2a') (1, σ2c') φ E)%I
+      (λ σ2a σ2c, wp_proc_seq_refinement Λa Λc (esa (Recovered (existT _ tt)))
+                                         (esc (Recovered (existT _ tt)))
+                                         rec (1, σ2a) (1, σ2c) φ E) E O
+  | _, _ => False%I
   end.
 
 Lemma crash_step_snd {OpT} (Λa: Layer OpT) σ1a σ2a t n:
@@ -102,14 +106,14 @@ Proof.
   eapply lifted_finish_step_intro; eauto.
 Qed.
 
-Lemma wp_recovery_refinement_impl_wp_recovery {T R} OpTa OpTc Σ (Λa: Layer OpTa) (Λc: Layer OpTc)
+Lemma wp_recovery_refinement_impl_wp_recovery {Ta Tc R} OpTa OpTc Σ (Λa: Layer OpTa) (Λc: Layer OpTc)
         `{invPreG Σ} `{cfgPreG OpTa Λa Σ}
-        (ea: proc OpTa T) (ec: proc OpTc T) (rec: proc OpTc R) σ1a σ1c φ φrec E k
+        (ea: proc OpTa Ta) (ec: proc OpTc Tc) (rec: proc OpTc R) σ1a σ1c φ φrec E k
         (Hno_fault : ¬ exec Λa ea (1, σ1a) Err):
   wp_recovery_refinement Σ Λa Λc ea ec rec (1, σ1a) σ1c φ φrec E k ⊢
   wp_recovery NotStuck ec rec σ1c
-    (λ (v : T) (σ2c : State Λc),
-       ∃ σ2a, ⌜exec Λa ea (1, σ1a) (Val σ2a (existT T v))⌝ ∗ φ v σ2a.2 σ2c.2)
+    (λ (vc : Tc) (σ2c : State Λc),
+       ∃ va σ2a, ⌜exec Λa ea (1, σ1a) (Val σ2a (existT Ta va))⌝ ∗ φ va vc σ2a.2 σ2c.2)
     (λ σ2c : State Λc,
        ∃ tp2 (σ2a σ2a' : Proc.State),
          ⌜exec_partial Λa ea (1, σ1a) (Val σ2a tp2) ∧ lifted_crash_step Λa σ2a (Val σ2a' tt)⌝
@@ -118,7 +122,7 @@ Proof.
   iIntros "Hwp".
   iApply (bupd_iter_mono with "[] Hwp"). iIntros "Hwp".
   iDestruct "Hwp" as (Hclosure φinv) "Hwp".
-  iExists (fun σ => (∃ _ : cfgG Σ, φinv _ σ ∗ source_inv [existT T ea] (σ1a))%I).
+  iExists (fun σ => (∃ _ : cfgG Σ, φinv _ σ ∗ source_inv [existT Ta ea] (σ1a))%I).
   iIntros (Hinv).
   assert (Inhabited Λa.(OpState)).
   { eexists; eauto. } (* econstructor. exact O. exact σ1a. } *)
@@ -131,7 +135,8 @@ Proof.
   }
   iExists stateI. iIntros "{$Hstate} !>".
   iSplitL "H"; last iSplitL "Hinv".
-  * iApply wp_wand_l; iFrame "H". iIntros (v') "[Hmapsto Hopen]".
+  * iApply wp_wand_l; iFrame "H". iIntros (vc) "H".
+    iDestruct "H" as (va) "(Hmapsto&Hopen)".
     iIntros (σ2c') "Hstate".
     iMod ("Hopen" with "Hstate") as (σ2a) "(Hstate&Habsr)".
     iInv "Hsrc" as (tp' n' σ') ">[Hauth Hp]" "_".
@@ -141,7 +146,7 @@ Proof.
     apply take_drop_middle in Hlookup.
 
     iApply fupd_mask_weaken; first by set_solver+.
-    iExists (n', σ'). iSplit; auto. iPureIntro. 
+    iExists va, (n', σ'). iSplit; auto. iPureIntro. 
     rewrite -Hlookup //= /of_val in Hp.
     eapply exec_partial_finish; eauto.
   * iIntros. iMod ("Hinv" with "[$]").
@@ -177,14 +182,15 @@ Proof.
        iFrame. iExists _; iFrame.
 Qed.
 
-Theorem wp_recovery_refinement_adequacy_internal {T R} OpTa OpTc Σ (Λa: Layer OpTa) (Λc: Layer OpTc)
+Theorem wp_recovery_refinement_adequacy_internal {Ta Tc R} OpTa OpTc Σ
+        (Λa: Layer OpTa) (Λc: Layer OpTc)
         `{invPreG Σ} `{cfgPreG OpTa Λa Σ}
-        (ea: proc OpTa T) (ec: proc OpTc T) (rec: proc OpTc R) σ1a σ1c φ φrec E k
+        (ea: proc OpTa Ta) (ec: proc OpTc Tc) (rec: proc OpTc R) σ1a σ1c φ φrec E k
         (Hno_fault : ¬ exec Λa ea (1, σ1a) Err):
   wp_recovery_refinement Σ Λa Λc ea ec rec (1, σ1a) σ1c φ φrec E k ⊢
   recv_adequate_internal NotStuck ec rec σ1c
-    (λ v σ2c, ∃ σ2a, ⌜ exec Λa ea (1, σ1a) (Val σ2a (existT _ v)) ⌝
-                            ∗ φ v (snd σ2a) (snd σ2c))%I
+    (λ v σ2c, ∃ va σ2a, ⌜ exec Λa ea (1, σ1a) (Val σ2a (existT _ va)) ⌝
+                            ∗ φ va v (snd σ2a) (snd σ2c))%I
     (λ σ2c, ∃ tp2 σ2a σ2a', ⌜ exec_partial Λa ea (1, σ1a) (Val σ2a tp2) ∧
                             lifted_crash_step Λa σ2a (Val σ2a' tt) ⌝ ∗ φrec (snd σ2a') (snd σ2c))%I k.
 Proof.
@@ -193,25 +199,37 @@ Proof.
   iApply wp_recovery_refinement_impl_wp_recovery; eauto.
 Qed.
 
-Theorem wp_proc_seq_refinement_adequacy_internal {T R} OpTa OpTc Σ (Λa: Layer OpTa) (Λc: Layer OpTc)
+Theorem wp_proc_seq_refinement_adequacy_internal {Ta Tc R} OpTa OpTc Σ (Λa: Layer OpTa) (Λc: Layer OpTc)
         `{invPreG Σ} `{cfgPreG OpTa Λa Σ}
-        (es: proc_seq OpTa T) (rec: proc OpTc R) f σ1c σ1a
-        φ E k
-        (Hno_fault : ¬ proc_exec_seq Λa es (rec_singleton (Ret tt)) (1, σ1a) Err):
-  Nat.iter k (λ P, |==> ▷ P)%I (wp_proc_seq_refinement Λa Λc es rec f (1, σ1a) σ1c φ E) ⊢
-  (∀ n σ2c res, ⌜proc_exec_seq_n Λc (map_proc_seq f es) rec n σ1c (Val σ2c res)⌝ →
+        (esa: proc_seq OpTa Ta) (esc: proc_seq OpTc Tc) (rec: proc OpTc R) σ1c σ1a
+        φ P E k
+        (Hno_fault : ¬ proc_exec_seq Λa esa (rec_singleton (Ret tt)) (1, σ1a) Err)
+        (Hφ: ∀ va vc σ2a σ2c, φ va vc σ2c σ2a -∗ ⌜ P va vc ⌝):
+  Nat.iter k (λ P, |==> ▷ P)%I (wp_proc_seq_refinement Λa Λc esa esc rec (1, σ1a) σ1c φ E) ⊢
+  (∀ n σ2c vc, ⌜proc_exec_seq_n Λc esc rec n σ1c (Val σ2c vc)⌝ →
                 (Nat.iter (S k + n) (λ P, |==> ▷ P)%I
-                          (⌜ ∃ σ2a, proc_exec_seq Λa es (rec_singleton (Ret tt))
-                                                       (1, σ1a) (Val σ2a res) ⌝ : iProp Σ))%I).
+                          (⌜ ∃ va σ2a, proc_exec_seq Λa esa (rec_singleton (Ret tt))
+                                                       (1, σ1a) (Val σ2a va) ∧ P va vc ⌝
+                                       : iProp Σ))%I).
 Proof.
   iIntros "Hwp". iIntros (n σ2c res Hexec). iRevert "Hwp".
-  iInduction es as [] "IH" forall (k n σ1c σ1a Hno_fault Hexec); iIntros "Hwp".
-  - iApply (@bupd_iter_le _ O) => //=; first by lia.
-    iPureIntro. destruct Hexec as (?&Hpure). inversion Hpure; subst.
-    exists (1, σ1a). econstructor.
-  - destruct Hexec as (n1&n2&Heq&(res0&σ1'&Hhd&Hrest)).
+  iInduction esa as [] "IH" forall (k n esc σ1c σ1a Hno_fault Hexec); iIntros "Hwp".
+  - destruct esc.
+    * iApply (@bupd_iter_le _ k) => //=; try lia.
+      iApply bupd_iter_mono; last eauto.
+      iIntros "H". iDestruct (Hφ with "H") as %?.
+      iPureIntro. destruct Hexec as (?&Hpure). inversion Hpure; subst.
+      eexists _, (1, σ1a). split; eauto. econstructor.
+    * iApply (@bupd_iter_le _ k) => //=; try lia.
+      iApply bupd_iter_mono; last eauto. auto.
+  - destruct esc.
+    { simpl.
+      iApply (@bupd_iter_le _ k) => //=; try lia.
+      iApply bupd_iter_mono; last eauto. auto.
+    }
+    destruct Hexec as (n1&n2&Heq&(res0&σ1'&Hhd&Hrest)).
       destruct Hhd as [Hnorm|Hrecv].
-      ** destruct Hnorm as (v&(?&?)&Hexec&Hfinish). 
+      ** destruct Hnorm as (v&(?&?)&Hexec&Hfinish).
          destruct Hfinish as ([]&(?&?)&Hfinish&Hpure).
          destruct Hfinish as ([]&(?&?)&Hputs&Hfinish).
          inversion Hputs; subst.
@@ -228,7 +246,7 @@ Proof.
 
          iIntros "H".
          iDestruct "H" as (v' Hp) "H". subst.
-         iDestruct "H" as (σ2a Hexeca) "H".
+         iDestruct "H" as (va σ2a Hexeca) "H".
          unshelve (iDestruct ("H" $! _ _) as (σ2a' Hfinisha) "H"); [| eauto|]; [].
          inversion H1; subst.
          iMod ("IH" $! _ O n2 with "[] [] H") as "H".
@@ -246,14 +264,14 @@ Proof.
          iNext.
          iApply bupd_iter_mono; last by iApply "H".
          iIntros "H".
-         iDestruct "H" as (σ2a'') "%".
-         iPureIntro. exists σ2a''.
+         iDestruct "H" as (va'' σ2a'') "(%&%)".
+         iPureIntro. exists va'', σ2a''; split; auto.
          do 2 eexists; split; eauto.
          left. do 2 eexists; split; eauto.
          eexists tt, _. split; eauto.
          eapply lifted_finish_step_intro'; eauto.
          econstructor.
-      ** destruct Hrecv as ([]&(?&?)&Hrexec&Hfinish). 
+      ** destruct Hrecv as ([]&(?&?)&Hrexec&Hfinish).
          destruct Hfinish as ([]&(?&?)&Hputs&Hpure).
          inversion Hpure. subst.
          destruct Hputs as (Hput&Hpure'). inversion Hpure'. subst.
@@ -285,8 +303,8 @@ Proof.
          iNext.
          iApply bupd_iter_mono; last by iApply "H".
          iIntros "H".
-         iDestruct "H" as (σ2a') "%".
-         iPureIntro. exists σ2a'.
+         iDestruct "H" as (va' σ2a') "(%&%)".
+         iPureIntro. exists va', σ2a'; split; auto.
          do 2 eexists; split; eauto.
          right.
          econstructor; last econstructor.
@@ -296,25 +314,27 @@ Proof.
          destruct σ2a; econstructor; eauto.
 Qed.
 
-Theorem wp_proc_seq_refinement_impl_wp_proc_seq {T R} OpTa OpTc Σ (Λa: Layer OpTa) (Λc: Layer OpTc)
+Theorem wp_proc_seq_refinement_impl_wp_proc_seq {Ta Tc R} OpTa OpTc Σ
+        (Λa: Layer OpTa) (Λc: Layer OpTc)
         `{invPreG Σ} `{cfgPreG OpTa Λa Σ}
-        (es: proc_seq OpTa T) (rec: proc OpTc R) f σ1c σ1a φ E
-        (Hno_fault : ¬ proc_exec_seq Λa es (rec_singleton (Ret tt)) (1, σ1a) Err):
-  wp_proc_seq_refinement Λa Λc es rec f (1, σ1a) (1, σ1c) φ E ⊢
-  wp_proc_seq NotStuck (map_proc_seq f es) rec (1, σ1c)
-    (λ (v : T) (σ2c : State Λc), ∃ σ2a, φ v σ2a (1, σ2c.2)).
+        (esa: proc_seq OpTa Ta) (esc: proc_seq OpTc Tc) (rec: proc OpTc R) σ1c σ1a φ E
+        (Hno_fault : ¬ proc_exec_seq Λa esa (rec_singleton (Ret tt)) (1, σ1a) Err):
+  wp_proc_seq_refinement Λa Λc esa esc rec (1, σ1a) (1, σ1c) φ E ⊢
+  wp_proc_seq NotStuck esc rec (1, σ1c)
+    (λ (vc : Tc) (σ2c : State Λc), ∃ va σ2a, φ va vc σ2a (1, σ2c.2)).
 Proof.
-  revert σ1c σ1a Hno_fault.
-  induction es as [| ??? IH] => σ1c σ1a Hno_fault.
-  - simpl. eauto.
-  - rewrite /wp_proc_seq_refinement -/wp_proc_seq_refinement.
+  revert esc σ1c σ1a Hno_fault.
+  induction esa as [| ??? IH] => esc σ1c σ1a Hno_fault.
+  - destruct esc; simpl; eauto. iIntros "[]".
+  - destruct esc; first by (simpl; eauto; iIntros "[]").
+    rewrite /wp_proc_seq_refinement -/wp_proc_seq_refinement.
     iIntros "Hwp".
     iPoseProof (wp_recovery_refinement_impl_wp_recovery with "Hwp") as "Hwp".
     { intros Hexec. apply Hno_fault. do 2 left. do 2 left.
       by apply exec_partial_err_exec_err. }
     iApply wp_recovery_mono; last iApply "Hwp"; rewrite -/wp_proc_seq.
     * iIntros (??) "H".
-      iDestruct "H" as (σ2a Hexeca) "H".
+      iDestruct "H" as (va σ2a Hexeca) "H".
       iIntros.
       iDestruct ("H" $! _ Hfinish) as (σ2a' Hexeca') "H".
       simpl. iApply IH.
@@ -347,12 +367,13 @@ Proof.
       eauto.
 Qed.
 
-Theorem wp_proc_seq_refinement_impl_wp_proc_seq' {T R} OpTa OpTc Σ (Λa: Layer OpTa) (Λc: Layer OpTc)
+Theorem wp_proc_seq_refinement_impl_wp_proc_seq' {Ta Tc R} OpTa OpTc Σ
+        (Λa: Layer OpTa) (Λc: Layer OpTc)
         `{invPreG Σ} `{cfgPreG OpTa Λa Σ}
-        (es: proc_seq OpTa T) (rec: proc OpTc R) f σ1c σ1a φ E
-        (Hno_fault : ¬ proc_exec_seq Λa es (rec_singleton (Ret tt)) (1, σ1a) Err):
-  wp_proc_seq_refinement Λa Λc es rec f (1, σ1a) (1, σ1c) φ E ⊢
-  wp_proc_seq NotStuck (map_proc_seq f es) rec (1, σ1c) (λ _ _, True).
+        (esa: proc_seq OpTa Ta) (esc: proc_seq OpTc Tc) (rec: proc OpTc R) σ1c σ1a φ E
+        (Hno_fault : ¬ proc_exec_seq Λa esa (rec_singleton (Ret tt)) (1, σ1a) Err):
+  wp_proc_seq_refinement Λa Λc esa esc rec (1, σ1a) (1, σ1c) φ E ⊢
+  wp_proc_seq NotStuck esc rec (1, σ1c) (λ _ _, True).
 Proof.
   iIntros "H".
   iPoseProof (wp_proc_seq_refinement_impl_wp_proc_seq with "H") as "H"; auto.
@@ -361,13 +382,16 @@ Proof.
 Qed.
 
 Import uPred.
+(* TODO: this can be generalized a bit to only require exact equality at
+   certain types *)
 Theorem wp_proc_seq_refinement_adequacy {T R} OpTa OpTc Σ (Λa: Layer OpTa) (Λc: Layer OpTc)
         `{invPreG Σ} `{cfgPreG OpTa Λa Σ}
-        (es: proc_seq OpTa T) (rec: proc OpTc R) f σ1c σ1a φ E
-        (Hno_fault : ¬ proc_exec_seq Λa es (rec_singleton (Ret tt)) (1, σ1a) Err):
-  wp_proc_seq_refinement Λa Λc es rec f (1, σ1a) (1, σ1c) φ E →
-  ∀ σ2c res, proc_exec_seq Λc (map_proc_seq f es) (rec_singleton rec) (1, σ1c) (Val σ2c res) →
-  ∃ σ2a, proc_exec_seq Λa es (rec_singleton (Ret tt)) (1, σ1a) (Val σ2a res).
+        (esa: proc_seq OpTa T) (esc: proc_seq OpTc T) (rec: proc OpTc R) σ1c σ1a φ E
+        (Hno_fault : ¬ proc_exec_seq Λa esa (rec_singleton (Ret tt)) (1, σ1a) Err)
+        (Hφ: ∀ va vc σ2a σ2c, φ va vc σ2c σ2a -∗ ⌜ va = vc ⌝):
+  wp_proc_seq_refinement Λa Λc esa esc rec  (1, σ1a) (1, σ1c) φ E →
+  ∀ σ2c res, proc_exec_seq Λc esc (rec_singleton rec) (1, σ1c) (Val σ2c res) →
+  ∃ σ2a, proc_exec_seq Λa esa (rec_singleton (Ret tt)) (1, σ1a) (Val σ2a res).
 Proof.
   intros Hwp ?? Hexec.
   eapply proc_exec_seq_equiv_proc_exec_seq_n in Hexec as (n&?); last first.
@@ -380,326 +404,11 @@ Proof.
   { eauto using lifted_crash_non_err. }
   eapply (soundness (M:=iResUR Σ) _ (S O + n)).
   iApply bupd_iter_laterN_mono; first by reflexivity; eauto.
-  iApply (wp_proc_seq_refinement_adequacy_internal); eauto.
-  iApply Hwp; eauto.
-Qed.
-
-(*
-Theorem wp_recovery_crash_refinement {T R} OpTa OpTc Σ (Λa: Layer OpTa) (Λc: Layer OpTc)
-        `{invPreG Σ} `{cfgPreG OpTa Λa Σ}
-        (ea: proc OpTa T) (ec: proc OpTc T) (rec: proc OpTc R)
-        (φinv : forall {_ : @cfgG OpTa Λa Σ}, Λc.(State) → iProp Σ)
-        (absr: forall _ : @cfgG OpTa Λa Σ, Λa.(State) → Λc.(State) → iProp Σ) E:
-  nclose sourceN ⊆ E →
-  (∀ (σ1a: Λa.(State)) σ1c,
-      (∀ `{Hinv : invG Σ} `{Hcfg: cfgG OpTa Λa Σ},
-          (absr _ σ1a σ1c) -∗
-          (|={⊤}=> ∃ stateI : State Λc → iProp Σ,
-             let _ : irisG OpTc Λc Σ := IrisG _ _ _ Hinv stateI in
-             (source_ctx ([existT _ ea], σ1a) ∗ O ⤇ ea ∗ source_state σ1a)
-               ={⊤}=∗
-               stateI σ1c
-               ∗ WP ec @ NotStuck; ⊤ {{ v, O ⤇ of_val v
-                    ∗ (∀ σ2c, stateI σ2c ={⊤,E}=∗ ∃ σ2a, source_state σ2a ∗ absr _ σ2a σ2c)}}
-                                     ∗ (∀ σ2c, stateI σ2c ={⊤,E}=∗ φinv σ2c)
-        ∗
-        □ (∀ `{Hinv : invG Σ} `{Hcfg: cfgG OpTa Λa Σ} σ1c σ1c'
-           (Hcrash: Λc.(crash_step) σ1c (Val σ1c' tt)),
-            (φinv σ1c ={⊤}=∗ ∃ stateI : State Λc → iProp Σ,
-               let _ : irisG OpTc Λc Σ := IrisG _ _ _ Hinv stateI in
-               stateI σ1c'
-               ∗ WP rec @ NotStuck; ⊤ {{ v, (∀ σ2c, stateI σ2c ={⊤,E}=∗
-                   ∃ σ2a σ2a', source_state σ2a ∗ ⌜Λa.(crash_step) σ2a (Val σ2a' tt) ⌝ ∗
-                               absr _ σ2a' σ2c)}}
-                                     ∗ (∀ σ2c, stateI σ2c ={⊤,E}=∗ φinv σ2c)))))%I) →
-  crash_refines (absr_to_iProp absr) Λc ec (rec_singleton rec) (Λa.(exec) ea)
-                (and_then (Λa.(exec_halt) ea) (fun _ => Λa.(crash_step))).
-Proof.
-  intros Hsub Hwp.
-  assert (Hno_fault_cut :
-            ∀ σ1a, ¬ (v <- exec Λa ea; _ <- (absr_to_iProp absr); pure v) σ1a Err ->
-                   ¬ exec Λa ea σ1a Err).
-  { clear. intros σ1a Hno_err.
-    intros Hexec. apply Hno_err.
-    left; auto.
-  }
-  assert (Hno_fault_cut':
-            ∀ σ1a, ¬ (v <- _ <- exec_halt Λa ea;
-                          Λa.(crash_step); _ <- (absr_to_iProp absr); pure v) σ1a Err ->
-                   ¬ exec Λa ea σ1a Err).
-  { clear. intros σ1a Hno_err.
-    intros Hexec. apply Hno_err. do 3 left. apply exec_partial_err_exec_err; eauto.
-  }
-  assert (Hadeq: ∀ σ1a σ1c (Hno_fault : ¬  exec Λa ea σ1a Err),
-             (absr_to_iProp absr σ1a (Val σ1c tt)) →
-             recv_adequate_internal (Σ := Σ) NotStuck ec rec σ1c
-                          (λ v' σ2c', ∃ H σ2a, ⌜ exec Λa ea σ1a (Val σ2a (existT _ v')) ⌝ ∗
-                                             absr H σ2a σ2c')%I
-                          (λ σ2c', ∃ H tp2 σ2a σ3a, ⌜ exec_partial Λa ea σ1a (Val σ2a tp2) ∧
-                                                      crash_step Λa σ2a (Val σ3a tt) ⌝ ∗
-                                                   absr H σ3a σ2c')%I).
-  { intros σ1a σ1c ? (k&Habsr_init).
-    eapply wp_recovery_adequacy_internal with
-        (φinv0 := fun σ => (∃ _ : cfgG Σ, φinv _ σ ∗ source_inv [existT T ea] σ1a)%I)
-        (k0 := k); eauto.
-    iIntros (Hinv).
-    assert (Inhabited Λa.(State)).
-    { eexists; eauto. }
-    iPoseProof Habsr_init as "Habsr_init".
-    iApply (bupd_iter_mono with "[] Habsr_init"). iClear "Habsr_init".
-    iIntros "Habsr_init".
-    iMod (source_cfg_init [existT _ ea] σ1a) as (cfgG) "(#Hsrc&Hpool&HstateA)"; auto.
-    { intros Herr; apply Hno_fault. apply exec_partial_err_exec_err; eauto. }
-    iPoseProof (Hwp _ _ with "Habsr_init") as "H".
-    iMod "H" as (stateI) "Hwand"; eauto.
-    iMod ("Hwand" with "[Hpool HstateA]") as "[Hstate [H [Hinv #Hφ]]]"; eauto.
-    { iFrame. iFrame "#".
-      rewrite /source_pool_map/tpool_to_map fmap_insert fmap_empty insert_empty //=.
-    }
-    iExists stateI. iIntros "{$Hstate} !>".
-    iSplitL "H"; last iSplitL "Hinv".
-    * iApply wp_wand_l; iFrame "H". iIntros (v') "[Hmapsto Hopen]".
-      iIntros (σ2c') "Hstate".
-      iMod ("Hopen" with "Hstate") as (σ2a) "(Hstate&Habsr)".
-      iInv "Hsrc" as (tp' σ') ">[Hauth Hp]" "_".
-      iDestruct "Hp" as %Hp. destruct Hp as (Hp&Hno_fault'). rewrite //= in Hp.
-      iDestruct (source_state_reconcile with "Hstate Hauth") as %Hstate; subst.
-      iDestruct (source_thread_reconcile with "Hmapsto Hauth") as %Hlookup; subst.
-      apply take_drop_middle in Hlookup.
-
-      iApply fupd_mask_weaken; first by set_solver+.
-      iExists _, σ'. iSplit; auto. iPureIntro. 
-      rewrite -Hlookup //= /of_val in Hp.
-      eapply exec_partial_finish; eauto.
-    * iIntros. iMod ("Hinv" with "[$]").
-      iMod (inv_open_timeless with "Hsrc") as "(?&_)"; first by eassumption.
-      iApply fupd_mask_weaken; auto.
-      { set_solver+. }
-      iFrame. iExists _; iFrame.
-    * iModIntro. iIntros (????) "Hinv".
-      iDestruct "Hinv" as (cfgG') "(?&HcfgInv)".
-      iClear "Hsrc".
-      iMod ("Hφ" with "[//] [$]") as (stateI') "(Hstate&Hwp&Hinv)".
-      iMod (inv_alloc sourceN ⊤ (source_inv _ _) with "HcfgInv") as "#cfgInv".
-      iModIntro. iExists stateI'. iFrame.
-      iSplitL "Hwp".
-      ** iApply wp_wand_l; iFrame.
-         iIntros (_) "H1".
-         iIntros (σ) "Hstate".
-         iMod ("H1" with "[$]") as (σ2a σ3a) "(Hstate&Hp&Habsr)".
-         iDestruct "Hp" as %Hcrash.
-         iMod (inv_open_timeless with "cfgInv") as "(Hinv&_)"; first by eassumption.
-         iApply fupd_mask_weaken; auto.
-         { set_solver+. }
-         iDestruct "Hinv" as (tp' σ3a') "(Hauth&%&%)".
-         iDestruct (source_state_reconcile with "Hstate Hauth") as %Hstate; subst.
-         iExists _, _, _, _. iFrame. iPureIntro; intuition eauto.
-      ** iIntros. iMod ("Hinv" with "[$]").
-         iMod (inv_open_timeless with "cfgInv") as "(?&_)"; first by eassumption.
-         iApply fupd_mask_weaken; auto.
-         { set_solver+. }
-         iFrame. iExists _; iFrame.
-  }
-  split.
-  - rewrite /refines.
-    apply rimpl_alt.
-    intros σ1a [σ2c (T'&v) |] Hno_fault; last first.
-    {
-      intros Hfalse; exfalso.
-      destruct Hfalse as [|([]&?&?&?)]; eauto.
-      edestruct Hadeq; eauto.
-      eapply recv_adequate_internal_not_stuck; eauto.
-      apply exec_err_rexec_err; eauto.
-    }
-    intros ([]&σ1c&Habsr&Hexec).
-    edestruct Hadeq; eauto.
-    edestruct (recv_adequate_normal_result) as (v'&Heq_val&σ2a&HexecA&Habsr'); eauto.
-    do 3 eexists; eauto.
-    do 3 eexists; eauto.
-    rewrite Heq_val. econstructor.
-  - rewrite /refines.
-    apply rimpl_alt.
-    intros σ1a [σ2c [] |] Hno_fault; last first.
-    {
-      intros Hfalse; exfalso.
-      destruct Hfalse as [|([]&?&?&?)]; eauto.
-      { eapply Habsr_no_err; eauto. }
-      edestruct Hadeq; eauto.
-      eapply recv_adequate_not_stuck; eauto.
-    }
-    intros ([]&σ1c&Habsr&Hexec).
-    edestruct Hadeq; eauto.
-    edestruct (recv_adequate_result) as (tp2&σ2a&?&HexecA&HcrashA&Habsr'); eauto.
-    do 3 eexists; eauto.
-    do 3 eexists; eauto.
-    * unshelve (do 3 eexists; eauto); try exact tt.
-      econstructor; eauto.
-    * unshelve (do 3 eexists; eauto); try exact tt.
-      econstructor; eauto.
-Qed.
-
-(* TODO: need to generalize so that φinv can depend on cfgG as above *)
-Theorem wp_recovery_trace_refinement {T R} OpTa OpTc Σ (Λa: Layer OpTa) (Λc: Layer OpTc)
-        `{invPreG Σ} `{cfgPreG OpTa Λa Σ}
-        (ea: proc OpTa T) (ec: proc OpTc T) (rec: proc OpTc R)
-        φinv (absr: relation Λa.(State) Λc.(State) unit) E
-        (Habsr_no_err: ∀ σa, ¬ absr σa Err):
-  nclose sourceN ⊆ E →
-  (∀ (σ1a: Λa.(State)) σ1c,
-      absr σ1a (Val σ1c tt) →
-      (∀ `{Hinv : invG Σ} `{Hcfg: cfgG OpTa Λa Σ},
-          (|={⊤}=> ∃ stateI : State Λc → iProp Σ,
-             let _ : irisG OpTc Λc Σ := IrisG _ _ _ Hinv stateI in
-             (source_ctx ([existT _ ea], σ1a) ∗ O ⤇ ea ∗ source_state σ1a)
-               ={⊤}=∗
-               stateI σ1c
-               ∗ WP ec @ NotStuck; ⊤ {{ v, O ⤇ of_val v
-                    ∗ (∀ σ2c, stateI σ2c ={⊤,E}=∗ ∃ σ2a, source_state σ2a ∗ ⌜absr σ2a (Val σ2c tt)⌝)}}
-                                      ∗ (∀ σ2c, stateI σ2c ={⊤,E}=∗ φinv σ2c
-                                                ∗ ∃ σ2a, source_state σ2a
-                                                     ∗ ⌜ trace_relation _ _ σ2a (Val σ2c tt) ⌝)
-        ∗
-        □ (∀ `{Hinv : invG Σ} `{Hcfg: cfgG OpTa Λa Σ} σ1c σ1c'
-           (Hcrash: Λc.(crash_step) σ1c (Val σ1c' tt)),
-            (φinv σ1c ={⊤}=∗ ∃ stateI : State Λc → iProp Σ,
-               let _ : irisG OpTc Λc Σ := IrisG _ _ _ Hinv stateI in
-               stateI σ1c'
-               ∗ WP rec @ NotStuck; ⊤ {{ v, (∀ σ2c, stateI σ2c ={⊤,E}=∗
-                   ∃ σ2a σ2a', source_state σ2a ∗ ⌜Λa.(crash_step) σ2a (Val σ2a' tt)
-                               ∧ absr σ2a' (Val σ2c tt)⌝)}}
-                                      ∗ (∀ σ2c, stateI σ2c ={⊤,E}=∗ φinv σ2c
-                                                ∗ ∃ σ2a, source_state σ2a
-                                                     ∗ ⌜ trace_relation _ _ σ2a (Val σ2c tt) ⌝)))))%I)
-    →
-  halt_refines absr Λc (trace_relation Λc Λa)
-                 ec
-                 (rec_singleton rec) (Λa.(exec_halt) ea)
-                 (and_then (Λa.(exec_halt) ea) (fun _ => Λa.(crash_step))).
-Proof.
-  intros Hsub Hwp.
-  apply halt_refines_trace_relation_alt; eauto.
-  rewrite /halt_refines/refines_if.
-  assert (Hno_fault_cut :
-            ∀ σ1a, ¬ (v <- exec Λa ea; _ <- absr; pure v) σ1a Err ->
-                   ¬ exec Λa ea σ1a Err).
-  { clear. intros σ1a Hno_err.
-    intros Hexec. apply Hno_err.
-    left; auto.
-  }
-  assert (Hno_fault_cut':
-            ∀ σ1a, ¬ (v <- _ <- exec_halt Λa ea;
-                          Λa.(crash_step); _ <- trace_relation Λc Λa; pure v) σ1a Err ->
-                   ¬ exec Λa ea σ1a Err).
-  { clear. intros σ1a Hno_err.
-    intros Hexec. apply Hno_err. do 3 left. apply exec_partial_err_exec_err; eauto.
-  }
-  apply rimpl_alt.
-  intros σ1a ret Hno_fault Hstep.
-  assert (∃ σ1c_outer,
-             absr σ1a (Val σ1c_outer ()) ∧
-             rexec_partial Λc ec (rec_singleton rec) σ1c_outer ret)
-         as (σ1c_outer&Habsr_init&Hexec).
+  iApply bupd_iter_mono; last first.
   {
-    destruct ret.
-    - destruct Hstep as ([]&?&?&?). eexists; split; eauto.
-    - destruct Hstep as [|([]&?&?&?)].
-      * exfalso. eapply Habsr_no_err; eauto.
-      * eauto.
+    iApply (wp_proc_seq_refinement_adequacy_internal); eauto.
+    iApply Hwp; eauto.
   }
-  edestruct @wp_recovery_invariance with
-        (ρ := fun σ2c => (v <- _ <- exec_halt Λa ea;
-            Λa.(crash_step); _ <- trace_relation Λc Λa; pure v) σ1a (Val σ2c ()))
-        (φ := fun (_ : T) (_ : Λc.(State)) => True)
-        (φrec := fun (_ : Λc.(State)) => True)
-        (φinv := fun σ => (φinv σ ∗ ∃ _ : cfgG Σ, source_inv [existT T ea] σ1a)%I)
-        as (Hρ&Hadeq); eauto.
-  {
-    iIntros (Hinv).
-    assert (Inhabited Λa.(State)).
-    { eexists; eauto. }
-    iMod (source_cfg_init [existT _ ea] σ1a) as (cfgG) "(#Hsrc&Hpool&HstateA)"; auto.
-    { intros Herr. eapply Hno_fault_cut'; first eapply Hno_fault.
-      apply exec_partial_err_exec_err; eauto. }
-    iPoseProof (Hwp _ _ Habsr_init $! Hinv cfgG) as "H".
-    iMod "H" as (stateI) "Hwand"; eauto.
-    iMod ("Hwand" with "[Hpool HstateA]") as "[Hstate [H [Hinv #Hφ]]]"; eauto.
-    { iFrame. iFrame "#".
-      rewrite /source_pool_map/tpool_to_map fmap_insert fmap_empty insert_empty //=.
-    }
-    iExists stateI. iIntros "{$Hstate} !>".
-    iSplitL "H"; last iSplitL "Hinv".
-    * iApply wp_wand_l; iFrame "H". iIntros (v') "[Hmapsto Hopen]".
-      iIntros (σ2c') "Hstate".
-      iMod ("Hopen" with "Hstate") as (σ2a) "(Hstate&%)".
-      iInv "Hsrc" as (tp' σ') ">[Hauth Hp]" "_".
-      iDestruct "Hp" as %Hp. destruct Hp as (Hp&Hno_fault'). rewrite //= in Hp.
-      iDestruct (source_state_reconcile with "Hstate Hauth") as %Hstate; subst.
-      iDestruct (source_thread_reconcile with "Hmapsto Hauth") as %Hlookup; subst.
-      apply take_drop_middle in Hlookup.
-
-      iApply fupd_mask_weaken; first by set_solver+.
-      iPureIntro; auto.
-    * iIntros.
-      iMod ("Hinv" with "[$]") as "(Hφinv&Hrest)".
-      iDestruct "Hrest" as (σ2a) "(Hstate&Htrace)". iDestruct "Htrace" as %Htrace.
-      iMod (inv_open_timeless with "Hsrc") as "(Hinv&_)"; first by eassumption.
-      iApply fupd_mask_weaken; auto.
-      { set_solver+. }
-      iDestruct "Hinv" as (tp' σ3a') "(Hauth&%&%)".
-      iDestruct (source_state_reconcile with "Hstate Hauth") as %Hstate; subst.
-      iFrame. iSplit.
-      ** iExists _, _; eauto.
-      ** iPureIntro.
-         edestruct (crash_total _ σ3a') as (σ3a''&?).
-         do 3 eexists.
-         { do 3 eexists; eauto.
-           do 3 eexists; eauto.
-           econstructor; eauto.
-         }
-         eexists tt, _; split; last by econstructor.
-         eexists; split; eauto.
-         transitivity (trace_proj _ σ3a').
-         { symmetry. eapply crash_preserves_trace; eauto. }
-         { inversion Htrace as (?&Heq&?). inversion Heq; subst; eauto. }
-    * iModIntro. iIntros (????) "(?&Hinv)".
-      iDestruct "Hinv" as (cfgG') "HcfgInv".
-      iClear "Hsrc".
-      iMod ("Hφ" with "[//] [$]") as (stateI') "(Hstate&Hwp&Hinv)".
-      iMod (inv_alloc sourceN ⊤ (source_inv _ _) with "HcfgInv") as "#cfgInv".
-      iModIntro. iExists stateI'. iFrame.
-      iSplitL "Hwp".
-      ** iApply wp_wand_l; iFrame.
-         iIntros (_) "H1".
-         iIntros (σ) "Hstate".
-         iMod ("H1" with "[$]") as (σ2a σ3a) "(Hstate&Hp)".
-         iDestruct "Hp" as %(Hcrash&Habsr).
-         iMod (inv_open_timeless with "cfgInv") as "(Hinv&_)"; first by eassumption.
-         iApply fupd_mask_weaken; auto.
-         { set_solver+. }
-      ** iIntros.
-         iMod ("Hinv" with "[$]") as "(Hφinv&Hrest)".
-         iDestruct "Hrest" as (σ2a) "(Hstate&Htrace)". iDestruct "Htrace" as %Htrace.
-         iMod (inv_open_timeless with "cfgInv") as "(Hinv&_)"; first by eassumption.
-         iApply fupd_mask_weaken; auto.
-         { set_solver+. }
-         iDestruct "Hinv" as (tp' σ3a') "(Hauth&%&%)".
-         iDestruct (source_state_reconcile with "Hstate Hauth") as %Hstate; subst.
-         iFrame. iSplit.
-         *** iExists _, _; eauto.
-         *** iPureIntro.
-         edestruct (crash_total _ σ3a') as (σ3a''&?).
-         do 3 eexists.
-         { do 3 eexists; eauto.
-           do 3 eexists; eauto.
-           econstructor; eauto.
-         }
-         eexists tt, _; split; last by econstructor.
-         eexists; split; eauto.
-         transitivity (trace_proj _ σ3a').
-         { symmetry. eapply crash_preserves_trace; eauto. }
-         { inversion Htrace as (?&Heq&?). inversion Heq; subst; eauto. }
-  }
-  destruct ret as [? []|]; eauto.
-  exfalso. eapply recv_adequate_not_stuck; eauto using rexec_partial_err_rexec_err.
+  iIntros "H". iDestruct "H" as %(va&σ2a&Hexec&Heq).
+  subst. eauto.
 Qed.
-*)
